Remove an admit on lowering condition

src/drf/Lift.v
@@ -107,12 +107,48 @@ Proof.
   - erewrite Memory.lower_o; eauto. condtac; ss. des; congr.
 Qed.
 
+Definition loc_ord_dec (loc:Loc.t) (ord:Ordering.t) (l:Loc.t):
+  {l = loc \/ Ordering.le ord Ordering.relaxed} + {~ (l = loc \/ Ordering.le ord Ordering.relaxed)}.
+Proof.
+  destruct (Loc.eq_dec l loc).
+  { left. auto. }
+  destruct (Ordering.le ord Ordering.relaxed) eqn:X.
+  { left. auto. }
+  right. contradict n. des; auto. congr.
+Defined.
+
+Definition Capability_lift_if loc ord l t rel :=
+  if loc_ord_dec loc ord l then rel else Capability_lift l t rel.
+
+Lemma Capability_lift_if_wf loc ord l t rel
+      (WF: Capability.wf rel):
+  Capability.wf (Capability_lift_if loc ord l t rel).
+Proof.
+  unfold Capability_lift_if. condtac; auto.
+  apply Capability_lift_wf. auto.
+Qed.
+
+Lemma Capability_lift_if_incr loc ord l t rel:
+  Capability.le rel (Capability_lift_if loc ord l t rel).
+Proof.
+  unfold Capability_lift_if. condtac; [refl|].
+  apply Capability_lift_incr.
+Qed.
+
+Lemma Capability_lift_if_mon loc ord l t rel1 rel2
+      (LE: Capability.le rel1 rel2):
+  Capability.le (Capability_lift_if loc ord l t rel1) (Capability_lift_if loc ord l t rel2).
+Proof.
+  unfold Capability_lift_if. condtac; auto.
+  apply Capability_lift_mon. auto.
+Qed.
+
 Definition pi_step_lift_mem l t p k (e:ThreadEvent.t) M1 M2 : Prop :=
   match ThreadEvent.is_writing e with
   | Some (loc,from,to,val,rel,ord) =>
     <<NOPRM: Memory.get loc to p = None>> /\
     <<DISJ: forall t' v' r' (KIND: k = Memory.promise_kind_split t' v' r'), Memory.get loc t' p = None>> /\
-    <<PMREL: Memory_op M1 loc from to val (if Loc.eq_dec l loc then rel else Capability_lift l t rel) M2 k>>
+    <<PMREL: Memory_op M1 loc from to val (Capability_lift_if loc ord l t rel) M2 k>>
   | None =>
     M1 = M2
   end.
@@ -323,58 +359,30 @@ Proof.
 Qed.
 
 Lemma mem_eqlerel_lower_forward
-      loc from to val released1 released2 released2'
+      loc from to val released1 released2
       m1 m2 m2'
       (MEMLE: mem_eqlerel m2 m1)
-      (LOWER2: Memory.lower m2 loc from to val released1 released2 m2')
-      (RELLE: Capability.le released2 released2')
-      (RELWF: Capability.wf released2'):
+      (LOWER2: Memory.lower m2 loc from to val released1 released2 m2'):
   exists released1' m1',
-    <<LOWER1: Memory.lower m1 loc from to val released1' released2' m1'>> /\
+    <<LOWER1: Memory.lower m1 loc from to val released1' released2 m1'>> /\
     <<MEMLE': mem_eqlerel m2' m1'>>.
 Proof.
   exploit Memory.lower_get0; eauto. i.
   apply MEMLE in x0. des.
-  exploit (@Memory.lower_exists m1 loc from to val rel2 released2'); eauto;
+  exploit (@Memory.lower_exists m1 loc from to val rel2 released2); eauto;
     try by inv LOWER2; inv LOWER; eauto; try by committac.
-  { admit. (* we have to use something different than lower *) }
+  { etrans; eauto. inv LOWER2. inv LOWER. auto. }
   i. des.
   esplits; eauto.
   econs; esplits; ii; revert IN0.
   - erewrite Memory.lower_o; eauto. erewrite (@Memory.lower_o mem2); eauto.
     condtac; ss.
-    + i. des. inv IN0. esplits; eauto.
+    + i. des. inv IN0. esplits; eauto. refl.
     + eapply MEMLE.
   - erewrite Memory.lower_o; eauto. erewrite (@Memory.lower_o m2'); eauto.
     condtac; ss.
-    + i. des. inv IN0. esplits; eauto.
+    + i. des. inv IN0. esplits; eauto. refl.
     + eapply MEMLE.
-Admitted.
-
-Definition Capability_lift_if loc l t rel :=
-  if Loc.eq_dec l loc then rel else Capability_lift l t rel.
-
-Lemma Capability_lift_if_wf loc l t rel
-      (WF: Capability.wf rel):
-  Capability.wf (Capability_lift_if loc l t rel).
-Proof.
-  unfold Capability_lift_if. condtac; auto.
-  apply Capability_lift_wf. auto.
-Qed.
-
-Lemma Capability_lift_if_incr loc l t rel:
-  Capability.le rel (Capability_lift_if loc l t rel).
-Proof.
-  unfold Capability_lift_if. condtac; [refl|].
-  apply Capability_lift_incr.
-Qed.
-
-Lemma Capability_lift_if_mon loc l t rel1 rel2
-      (LE: Capability.le rel1 rel2):
-  Capability.le (Capability_lift_if loc l t rel1) (Capability_lift_if loc l t rel2).
-Proof.
-  unfold Capability_lift_if. condtac; auto.
-  apply Capability_lift_mon. auto.
 Qed.
 
 Lemma write_step_pi_step_lift_mem
@@ -421,11 +429,17 @@ Proof.
     + i. inv KIND. destruct (Memory.get loc t' (Local.promises lco)) as [[]|] eqn:X; auto.
       exfalso. eapply Memory.disjoint_get; try apply DISJ; eauto.
       hexploit Memory.split_get0; try exact PROMISES; eauto. i. des. eauto.
-  - exploit mem_eqlerel_lower_forward; eauto.
-    { apply Capability_lift_if_incr. }
-    i. des. esplits; eauto. i.
+  - exploit mem_eqlerel_lower_forward; eauto. i. des.
+    esplits; eauto. i.
     unfold pi_step_lift_mem. rewrite E. splits; cycle 2.
-    + econs 3; eauto.
+    + unfold Capability_lift_if. condtac; cycle 1.
+      { exfalso. apply n. right. clear COND.
+        destruct (Ordering.le ord Ordering.relaxed) eqn:Y; ss.
+        exploit ORD; eauto.
+        { by destruct ord; inv Y. }
+        i. des. congr.
+      }
+      econs 3; eauto.
     + destruct (Memory.get loc to (Local.promises lco)) as [[]|] eqn:X; auto.
       exfalso. eapply Memory.disjoint_get; try apply DISJOINT2; eauto. s.
       erewrite Memory.lower_o; eauto. condtac; ss. des; congr.
@@ -647,9 +661,9 @@ Lemma pi_step_lift_except_future
   <<TIMELE: TimeMap.le cT1.(Configuration.sc) cT2.(Configuration.sc)>>.
 Proof.
   assert (EQMEM2: mem_eqrel (Capability_lift_le l t (msg_add e msgs)) cT2.(Configuration.memory) M2).
-  { unfold mem_eqrel. splits.
-    - admit. (* mem_eqrel *)
-    - admit. (* mem_eqrel *)
+  { inv PI_STEP. unfold mem_eqrel. splits.
+    - ii. admit. (* mem_eqrel *)
+    - ii. admit. (* mem_eqrel *)
   }
   assert (IN2: Memory.get l t cT2.(Configuration.memory) <> None).
   { destruct (Memory.get l t (Configuration.memory cT1)) as [[? []]|] eqn:X; [|congr].
@@ -667,21 +681,26 @@ Proof.
     { inv WF. auto. }
     i. des. inv PMREL.
     + econs 1; eauto.
-      * eapply mem_eqrel_closed_capability; eauto. condtac; ss.
+      * eapply mem_eqrel_closed_capability; eauto.
+        unfold Capability_lift_if. condtac; ss.
         eapply Capability_lift_closed_capability; eauto.
-      * condtac; ss.
+      * unfold Capability_lift_if. condtac; ss.
         destruct t4. ss. unfold TimeMap_lift. condtac; ss.
+        exfalso. apply n. auto.
     + econs 2; eauto.
-      * eapply mem_eqrel_closed_capability; eauto. condtac; ss.
+      * eapply mem_eqrel_closed_capability; eauto.
+        unfold Capability_lift_if. condtac; ss.
         eapply Capability_lift_closed_capability; eauto.
-      * condtac; ss.
+      * unfold Capability_lift_if. condtac; ss.
         destruct t4. ss. unfold TimeMap_lift. condtac; ss.
+        exfalso. apply n. auto.
     + econs 3; eauto.
-      * eapply mem_eqrel_closed_capability; eauto. condtac; ss.
+      * eapply mem_eqrel_closed_capability; eauto.
+        unfold Capability_lift_if. condtac; ss.
         eapply Capability_lift_closed_capability; eauto.
-      * condtac; ss.
+      * unfold Capability_lift_if. condtac; ss.
         destruct t4. ss. unfold TimeMap_lift. condtac; ss.
-      * admit. (* capability le (lowering) *)
+        exfalso. apply n. auto.
   - inv PI_STEP0.
     eapply small_step_future; eauto.
     inv WF. auto.
